backup for belazy

CCDeconstructed/Classes.lean
@@ -14,30 +14,32 @@ attribute [simp,aesop norm unfold] Coe.coe
 class WellScopedness (α : Type) where
   WellScopedRec : Nat → α → Prop
   WellScoped := WellScopedRec 0
-  WellScoped_implies_WellScopedRec_0 :
-    WellScoped t → WellScopedRec 0 t
-  WellScopedRec_weaken :
-    m <= n →
-    WellScopedRec m t →
-    WellScopedRec n t
 
-attribute [simp,aesop norm unfold]
-  WellScopedness.WellScopedRec
-  WellScopedness.WellScoped
-attribute [aesop unsafe forward 50%]
-  WellScopedness.WellScoped_implies_WellScopedRec_0
-attribute [aesop unsafe forward 20%]
-  WellScopedness.WellScopedRec_weaken
+namespace WellScopedness
+  attribute [simp,aesop norm unfold] WellScopedRec WellScoped
+
+  class Infrastructure (α : Type) extends WellScopedness α where
+    WellScoped_implies_WellScopedRec_0 :
+      WellScoped t →
+      WellScopedRec 0 t
+    WellScopedRec_weaken :
+      m <= n →
+      WellScopedRec m t →
+      WellScopedRec n t
+end WellScopedness
 
 class FreeVariables (α : Type) (β : VarCat i) where
   fv : α → Finset (Atom β)
 
+namespace FreeVariables
+  attribute [simp,aesop norm unfold] fv
+
+  instance instAtom : FreeVariables (Atom α) α := ⟨singleton⟩
+  instance instFinsetAtom : FreeVariables (Finset (Atom α)) α := ⟨id⟩
+  instance instFinsetFreeVariables [FreeVariables α β] : FreeVariables (Finset α) β := ⟨fun s => s.fold (· ∪ ·) ∅ fv⟩
+end FreeVariables
+
 open FreeVariables
-
-attribute [simp,aesop norm unfold] FreeVariables.fv
-
-instance : FreeVariables (Atom α) α := ⟨singleton⟩
-instance : FreeVariables (Finset (Atom α)) α := ⟨id⟩
 
 @[simp,aesop norm unfold]
 def VarCat.type (α : VarCat i) : Type :=
@@ -47,51 +49,86 @@ def VarCat.type (α : VarCat i) : Type :=
 
 open VarCat
 
+class Scoped (α : Type) (β : VarCat i) extends FreeVariables α β where
+  instantiateRec : α → Index β → β.type → α
+  substitute : α → Atom β → β.type → α
+
+namespace Scoped
+  attribute [simp] instantiateRec substitute
+
+  @[simp]
+  def instantiate [Scoped α β] (t : α) (u : type β) : α :=
+    instantiateRec t 0 u
+
+  set_option synthInstance.checkSynthOrder false
+  class Infrastructure (α : Type) (β : VarCat i) extends Scoped α β, WellScopedness.Infrastructure α where
+    substitute_fresh :
+      x ∉ fv t →
+      substitute t x u = t
+    WellScopedRec_instantiateRec :
+      WellScopedRec n (instantiateRec t n u) →
+      WellScopedRec (n + 1) t
+    instantiateRec_WellScopedRec :
+      WellScopedRec n t →
+      k >= n →
+      instantiateRec t k u = t
+
+  @[simp]
+  lemma Instractructure.instantiateRec_WellScoped [self : Infrastructure α β] :
+    self.WellScoped t →
+    self.instantiateRec t k u = t
+  := by
+    intros H
+    apply self.instantiateRec_WellScopedRec
+    · apply self.WellScoped_implies_WellScopedRec_0 H
+    · linarith
+
+  attribute [aesop unsafe forward 20%]
+    Infrastructure.substitute_fresh
+    Infrastructure.instantiateRec_WellScopedRec
+    Infrastructure.WellScopedRec_instantiateRec
+end Scoped
+
 set_option synthInstance.checkSynthOrder false
-class Scoped (α : Type) (β : VarCat i) extends WellScopedness α, FreeVariables α β where
-  instantiateRec : α → Index β → type β → α
-  substitute : α → Atom β → type β → α
-  substitute_fresh :
-    x ∉ fv t →
-    substitute t x u = t
-  WellScopedRec_instantiateRec :
-    WellScopedRec n (instantiateRec t n u) →
-    WellScopedRec (n + 1) t
-  instantiateRec_WellScopedRec :
-    WellScopedRec n t →
-    k >= n →
-    instantiateRec t k u = t
-
-attribute [simp]
-  Scoped.instantiateRec
-  Scoped.substitute
-attribute [aesop unsafe forward 20%]
-  Scoped.substitute_fresh
-  Scoped.instantiateRec_WellScopedRec
-
-@[simp]
-def Scoped.instantiate [Scoped α β] (t : α) (u : type β) : α := instantiateRec t 0 u
-
-@[simp]
-lemma instantiateRec_WellScoped [s : Scoped α β] :
-  s.WellScoped t →
-  s.instantiateRec t k u = t
-:= by
-  intros H
-  apply s.instantiateRec_WellScopedRec
-  · apply s.WellScoped_implies_WellScopedRec_0 H
-  · linarith
-
 class WellFormedness (i : CC) (α : Type) extends WellScopedness α where
   WellFormed : Env i → α → Prop
   WellFormed_WellScoped :
     WellFormed Γ t →
     WellScoped t
   WellFormed_weaken :
-    WellFormed Δ t →
+    WellFormed (Γ ++ Δ) t →
+    Env.Nodup (Γ ++ Θ ++ Δ) →
+    WellFormed (Γ ++ Θ ++ Δ) t
+
+namespace WellFormedness
+  lemma WellFormed_weaken_head {i : CC} [self : WellFormedness i α] {Γ Δ : Env i} {t : α} :
+    WellFormed Γ t →
+    Env.Nodup (Γ ++ Δ) →
     WellFormed (Γ ++ Δ) t
-  WellFormed_weaken_head :
+  := by
+    intros WF Nodup
+    conv in Γ ++ Δ =>
+      rw [<- Env.concat_nil (Γ := Γ ++ Δ)]
+      rfl
+    apply WellFormed_weaken
+      <;> assumption
+
+  lemma WellFormed_weaken_cons {i : CC} [self : WellFormedness i α] {Γ : Env i} {a : Assoc i} {t : α} :
+    Env.Nodup Γ →
+    a.name ∉ Env.dom Γ →
     WellFormed Γ t →
     WellFormed (Γ ▷ a) t
   := by
-    apply WellForm
+    intros Nodup NotIn WF
+    rw [<- Env.concat_singleton]
+    apply WellFormed_weaken_head WF
+    apply Env.Nodup.cons Nodup NotIn
+end WellFormedness
+
+structure Scope {α : Type} (β : VarCat i) [Scoped α β] (P : α → Prop) (t : α) where
+  atoms : Finset (Atom β)
+  proof : ∀ x ∉ atoms, P (Scoped.instantiate (β := β) t
+    (match β with
+     | .var _ => .free x
+     | .tvar _ =>.var (.free x)
+    ))
