CCDeconstructed/Infrastructure/Var.lean
@@ -4,62 +4,63 @@ import CCDeconstructed.Classes
 open Scoped FreeVariables VarCat
 
 namespace Var
-  instance : Coe (Atom α) (Var α) where
+  instance {α : VarCat i} : Coe (Atom α) (Var α) where
     coe := Var.free
 
-  instance : Coe (Index α) (Var α) where
+  instance {α : VarCat i} : Coe (Index α) (Var α) where
     coe := Var.bound
 
   @[aesop norm]
-  def fv : Var α → Finset (Atom α)
+  def fv {α : VarCat i} : Var α → Finset (Atom α)
       | .free x => {x}
       | .bound _ => ∅
       | .cap => ∅
 
   @[aesop norm]
-  def bv : Var α → Finset (Index α)
+  def bv {α : VarCat i} : Var α → Finset (Index α)
     | .free _ => ∅
     | .bound i => {i}
     | .cap => ∅
 
   @[simp,aesop norm]
-  def subst [Coe (Var α) β] (v : Var α) (x : Var α) (u : β) : β :=
+  def subst {i : CC} {α : VarCat i} {β : Type} [Coe (Var α) β] (v : Var α) (x : Var α) (u : β) : β :=
     if v = x then u else v
 
   @[aesop norm]
-  def substitute {i} {α : VarCat i} (v : Var α) (x : Atom α) (u : Var α) : Var α :=
+  def substitute {i : CC} {α : VarCat i} (v : Var α) (x : Atom α) (u : Var α) : Var α :=
     @subst i α (Var α) ⟨id⟩ v (.free x) u
 
   @[aesop norm]
   def instantiateRec {i} {α : VarCat i} (v : Var α) (k : Index α) (u : Var α) : Var α :=
     @subst i α (Var α) ⟨id⟩ v (.bound k) u
 
+  @[simp]
   instance instFreeVariables : FreeVariables (Var α) α where
     fv := fv
 
   @[aesop norm]
-  def WellScopedRec {i : CC} {α : VarCat i} (allowCap := false) (n : Nat) : Var α → Prop
+  def WellScopedRec {i : CC} {α : VarCat i} {allowCap : Bool} (n : Nat) : Var α → Prop
     | .bound k => k < n
     | .free _ => True
     | .cap => if allowCap then True else False
 
   @[aesop norm]
-  def WellScoped {i : CC} {α : VarCat i} (allowCap := false) : Var α → Prop
+  def WellScoped {i : CC} {α : VarCat i} {allowCap : Bool} : Var α → Prop
     | .bound _ => False
     | .free _ => True
     | .cap => if allowCap then True else False
 
   @[aesop safe apply]
-  lemma WellScoped_implies_WellScopedRec_0 :
-    WellScoped allowCap t →
-    WellScopedRec allowCap 0 t
+  lemma WellScoped_implies_WellScopedRec_0 {i : CC} {α : VarCat i} {v : Var α} {allowCap : Bool} :
+    WellScoped (allowCap := allowCap) v →
+    WellScopedRec (allowCap := allowCap) 0 v
   := by simp [WellScoped,WellScopedRec]
 
   @[aesop safe apply]
-  lemma WellScopedRec_weaken :
+  lemma WellScopedRec_weaken {i : CC} {α : VarCat i} {v : Var α} {allowCap : Bool} :
     m <= n →
-    WellScopedRec allowCap m v →
-    WellScopedRec allowCap n v
+    WellScopedRec (allowCap := allowCap) m v →
+    WellScopedRec (allowCap := allowCap) n v
   := by
     simp [WellScopedRec]
     intros
@@ -68,11 +69,16 @@ namespace Var
     · case bound => simp [Index] at *; linarith
     · case cap => cases allowCap <;> simp at *
 
-  instance instWellScopedness (allowCap : Bool) : WellScopedness (Var α) where
-    WellScopedRec := WellScopedRec allowCap
-    WellScoped := WellScoped allowCap
-    WellScoped_implies_WellScopedRec_0 := WellScoped_implies_WellScopedRec_0
-    WellScopedRec_weaken := WellScopedRec_weaken
+  @[simp]
+  instance instWellScopedness (allowCap : Bool) {α : VarCat i} : WellScopedness (Var α) where
+    WellScoped := WellScoped (allowCap := allowCap)
+    WellScopedRec := WellScopedRec (allowCap := allowCap)
+
+  @[simp]
+  instance instWellScopednessInfrastructure (allowCap : Bool) {α : VarCat i} : WellScopedness.Infrastructure (Var α) where
+    toWellScopedness := instWellScopedness allowCap
+    WellScoped_implies_WellScopedRec_0 := WellScoped_implies_WellScopedRec_0 (allowCap := allowCap)
+    WellScopedRec_weaken := WellScopedRec_weaken (allowCap := allowCap)
 
   @[aesop safe apply]
   lemma substitute_fresh :
@@ -82,8 +88,8 @@ namespace Var
 
   @[aesop safe apply]
   lemma WellScopedRec_instantiateRec :
-    WellScopedRec allowCap n (instantiateRec v n u)→
-    WellScopedRec allowCap (n + 1) v
+    WellScopedRec (allowCap := allowCap) n (instantiateRec v n u) →
+    WellScopedRec (allowCap := allowCap) (n + 1) v
   := by
     simp [WellScopedRec]
     intros WS
@@ -91,7 +97,7 @@ namespace Var
     · case free => simp
     · case bound k =>
       simp [instantiateRec] at *
-      cases (decEq k n) <;> rename_i H <;> simp [H,Index] at *
+      cases decEq k n <;> rename_i H <;> simp [H,Index] at *
       linarith
     · case cap =>
       simp [instantiateRec] at *
@@ -99,7 +105,7 @@ namespace Var
 
   @[aesop safe apply]
   lemma instantiateRec_WellScopedRec :
-    WellScopedRec allowCap n v →
+    WellScopedRec (allowCap := allowCap) n v →
     k >= n →
     instantiateRec v k u = v
   := by
@@ -108,12 +114,28 @@ namespace Var
     cases v <;> simp [Index] at *
     case bound k => exfalso; linarith
 
+  @[simp]
   instance instScoped (allowCap : Bool) : Scoped (Var (.var i)) (.var i) where
     instantiateRec := instantiateRec
     substitute := substitute
-    substitute_fresh := substitute_fresh
-    WellScopedRec_instantiateRec := WellScopedRec_instantiateRec (allowCap := allowCap)
-    instantiateRec_WellScopedRec := instantiateRec_WellScopedRec (allowCap := allowCap)
-    WellScoped_implies_WellScopedRec_0 := WellScoped_implies_WellScopedRec_0
+
+  @[simp]
+  instance instScopedInfrastructure (allowCap : Bool) : Scoped.Infrastructure (Var (.var i)) (.var i) where
+    WellScopedRec := WellScopedRec
     WellScopedRec_weaken := WellScopedRec_weaken
+    WellScoped_implies_WellScopedRec_0 := WellScoped_implies_WellScopedRec_0
+    instantiateRec := instantiateRec
+    substitute := substitute
+    substitute_fresh := substitute_fresh
+    WellScopedRec_instantiateRec := by
+      intros n v u WS
+      simp [Scoped.instantiateRec] at *
+      apply WellScopedRec_instantiateRec (allowCap := allowCap)
+      apply WS
+    instantiateRec_WellScopedRec := by
+      intros n v m u WS leq
+      simp [Scoped.instantiateRec] at *
+      apply instantiateRec_WellScopedRec (allowCap := allowCap) (n := n) (u := u)
+      · apply WS
+      · apply leq
 end Var
